+++
title = "Replacement Rate"
date = 2025-02-07T22:24:15+09:00
math = true
+++

There has never beed so many people in the world.
Just a few decades ago, there was science fiction of future worlds, crowded with people.
Now it's ironically the opposite.
The fertility rate[^frate] is a common word.
It's commonly said that a fertility rate of 2.1 is needed to sustain a population.
I thought today would be a good opportunity to understand fertility rate andto understand this replacement rate.
First, I want to introduce a simple population mode
Second with that model, I want to try to understand the needed fertility rate to achieve a stable population.

[^frate]: The number of children a woman on average has in their lifetime.

# The Model

The model is simple, let's say we have a population that is divided up into age groups.
We can be as coarse or fine grained here.
I will work with time gradations years.
So people $t$ years old but not $t+1$ years old will be labeled as $P_t$.
I think it a bit easier to work with fraction of the total population instead, so let's take $p_t = P_t / P$ as number of people of a certain age as a fraction of the population.
Further more, let's introduce $b_t$ as the fraction of people give birth[^onegender] at age $t$.
$d_t$ is the fraction of people at age $t$ who perish before their next birthday.
Finally, it makes sense that people cannont have babies right after birth so let's have a minimum age at which people can start giving birth, $t_b$.

[^onegender]: My world here has only one gender.

<!-- The aim of $b_t$ is to be related to the fertility rate such that, $\sum_{t=0} b_t = B$. -->

Let's introduce the dynamic part of the model.
The age groups the next year is related to the previous poplutaion as the following.

\begin{equation}
 \tilde P_{t+1} = (1 - d_t) P_{t} \text{ where } t > 0
\end{equation}

\begin{equation}
 \tilde P_{0} = \sum_{t = t_b} b_t P_{t}
\end{equation}

# Analysis

## Fertility rate

It would be nice to relate our $b$ to fertility rate, $B$.
Taking the definition of fertility rate[^frate], we find that it can be caculated as the average of a single person over their entire life.
Since we know the rate of death and birth we can find chance a person lives to a certain age.
Nowing the change a person lives to a certain age, we can then perform the average.
So we can defined $y_t$ as the probability a person lives to $y_t$ and dies before their next birthday.

For $y_0 = d_0$.
For $y_1 = (d_0-1) d_1$.
For $y_2 = (d_0-1) (d_1-1) d_2$.
Seeing a pattern we can write $y_t =  d_t\prod_{s = 1}^{t-1} (1 - d_s)$.
As long as $\forall t, |1 - d_t| < 1$ <!-- > -->, $y$ over $t$ can be normalized as a probability distribution.

Let's take the case where $d_t = d$, a constant value.
So $y_t = d(1 - d)^t$ otherwise.

Now let's normalize by $\sum_t y_t = \sum_t d (1 - d)^t = 1$.
Serendipitously, $y$ is already normalized!
Let's call it $\hat y$ to remind outselves of this fact.
<!-- The actual probabilities being $\hat y_0 = d/(1+d)$ and $\hat y_t = d(1 - d)^{t-1}/(1+d)$. -->
So now we will calculate the average number of babies a person has, averaging over every possibility.

 <!-- B = \sum_t \sum_{s=t_b}^t b_s \hat y_t = \frac d{1+d}\sum_{t=t_b} \sum_{s=t_b}^t b_s (1 - d)^{t-1} -->
\begin{equation}
 B = \sum_t \sum_{s=t_b}^t b_s \hat y_t = \sum_{t=t_b} \sum_{s=t_b}^t b_s d (1 - d)^t
\end{equation}

We could take $b_t = b$ to be constant here too with respect to age, so we get

 <!-- B =  \frac {bd}{1+d}\sum_{t=t_b} (t-t_b+1) (1 - d)^{t-1} = \frac {bd}{1+d}\sum_{r=0} (r+1) (1 - d)^{r+t_b-1} -->
\begin{equation}
 B =  bd\sum_{t=t_b} (t-t_b+1) (1 - d)^t = bd\sum_{r=0} (r+1) (1 - d)^{ r + t_b }
\end{equation}

So we get 

 <!-- B = \frac {b(1-d)^{t_b-1}}{d(1+d)} -->
\begin{equation}
 B = b \frac{(1-d)^{t_b}}{d}
\end{equation}

It makes sence that $b=0$ means not births and for $d\to0$ we have a divergence to positive infinity.
We can also calculate the average age lived too.

 <!-- D = \sum_t t \hat y_t = \frac d{1+d}\sum_{t=1} t (1 - d)^{t-1} = \frac 1{d( 1+d )} -->
\begin{equation}
 D = \sum_t t \hat y_t = d \sum_t t (1-d)^t = \frac {1-d}d
\end{equation}

I will leave to the reader to express $d$ and $b$ in terms of $D$ and $B$.
<!-- Also, for the case where $t_b = 0$, I leave to the reader. -->

<!-- d = 1 / (1+D) -->
<!-- b = B (1+D)^{t_b - 1}/D^{t_b} -->

## Replacement Rate

From the last section, ingeneral for large $B$ and low $D$, in general the population increases.
If these are too low, the population cannot sustain itself.
What is the sweet spot where the population does not increase nor decrease?
Said in another way, what should $B$ give $D$ so the population is stable?

To most straight forward way is to use the dynamic equation we postulated with an addtion contraints that the population does not change, ie $\tilde P = P$.
Maybe a more strict conditions is that every age groups does not change.
It's like all the people who age out of an age group (or die out) is equal to the amount of people how age into it.
For age $0$, the people entering are those being born.
Essentially, $\tilde P_t = P_t$.
So we that make a system of equations for $P$!

\begin{equation}
 P_{t+1} = (1 - d_t) P_{t} \text{ where } t > 0
\end{equation}

\begin{equation}
 P_{0} = \sum_{t = t_b} b_t P_{t}
\end{equation}

For simplicity let's assume again that $d_t$ is one value.
Looking at the case of $t>0$ for a few $t$'s.
We get  
$P_{1} = (1-d) P_0$,  
$P_{2} = (1-d)^2 P_0$, and  
$P_{3} = (1-d)^3 P_0$.  

So at least for $t>0$, we can solve recusively for $P_t = (1-d)^t P_0$.
Now we can plug that into our $P_0$ equation (assuming again like before that $b_r = b$)!

\begin{equation}
 P_{0} = b \sum_{t = t_b} (1-d)^t P_0 = P_0 \frac{b (1-d)^{t_b}}{d} 
\end{equation}

Solving for $d$, we get $b = \frac{d}{(1-d)^{t_b}}$.
This implies for $B$

\begin{equation}
 B = \frac{d}{(1-d)^{t_b}} \frac{(1-d)^{t_b}}{d} = 1
\end{equation}

Thinking about this result, it makes sense. Every one need to replaces themselves on average.
If we consider the case where have the population cannont give birth, $b \to b/2$.
The $B$ becomes $2$.
So, who to people get to the $2.1$ figure?
We could also $1/2.1$ fraction of the population cannont give birth, but that seems like a cop out.
Maybe next time we can make a better model.
Or maybe the reader can?

<!-- Let's try making the bith part of our model more complicated. -->
<!-- Let's add the fact that women cannot give birth forever, since they have a finte about of eggs there is an age from after reproduction becomes impossible. -->

<!-- ## Adding a brith age limit -->

<!-- So, to account for this let's say that after some age $t_s$, birth stops person ie for $t > t_s$ $b_t = 0$. -->
<!-- Doing this changes our $B$ to the following -->

<!-- \begin{equation} -->
<!--  B = \frac{b}{d} \left( (d-1) (1-d)^{t_s} (d (t_s-t_b+1)+1)+(1-d)^{t_b} \right) \text{ for } t_s \geq t_b -->
<!-- \end{equation} -->

<!-- Now equilibrium implies that --> 

<!-- \begin{equation} -->
<!--  P_{0} = b \sum_{t = t_b}^{t_s} (1-d)^t P_0 = P_0 b \frac{(1-d)^{t_b}-(1-d)^{t_s+1}}{d} -->
<!-- \end{equation} -->

<!-- This implies that -->

<!-- \begin{equation} -->
<!--  b = \frac{d}{(1-d)^{t_b}-(1-d)^{t_s+1}} -->
<!-- \end{equation} -->

<!-- which implies for $B$ that -->

<!-- \begin{equation} -->
<!--  B = \frac{(d-1) (1-d)^{t_s} (d (t_s-t_b+1)+1)+(1-d)^{t_b}}{(1-d)^{t_b}-(1-d)^{t_s+1}} \text{ for } t_s \geq t_b -->
<!-- \end{equation} -->

<!-- \begin{equation} -->
<!--  B = (1-d)^{t_b} \left( (d-1) (1-d)^{t_s} (d (t_s-t_b+1)+1)+(1-d)^{t_b} \right) \text{ for } t_s \geq t_b -->
<!-- \end{equation} -->


<!-- For replacement rate we want to know the equilibrium point... -->

<!-- makePeqs[maxage_, birthage_] := Table[C[n+1] == (1-dr) C[n], {n, 0, maxage}] ~Join~ {C[0] == Sum[br C[n], {n, birthage, maxage}], Sum[C[n], {n, 0, maxage}] == 1} --> 

<!-- function makepop(maxage, birthage, dr, fertrate; T = Float64) -->
<!--            br = fertrate / (maxage - birthage + 1) -->
<!--            m = zeros(T, maxage + 1, maxage + 1) -->
<!--            # pâ€²j = mji pi -->
<!--            for ((j, agej), (i, agei)) in Iterators.product(enumerate(0:maxage), enumerate(0:maxage)) -->
<!--                if i + 1 == j -->
<!--                    m[j, i] = (1 - dr) -->
<!--                end -->
       
<!--                if agei >= birthage && agej == 0 -->
<!--                    m[j, i] = br -->
<!--                end -->
<!--            end -->
<!--            return m -->
<!--        end -->
